tests/lean/grind/congruence_hint.lean
@@ -10,4 +10,4 @@ trace: [grind.hints] Hints
 -/
 #guard_msgs in
 example (f : Nat → Nat) (y z : Nat) (h : y = z) : f y = f z := by
-  grind
+  grind??
